par_body_n__Sn

swotarfe_andufotions/src/Smallstep.v
@@ -688,3 +688,208 @@ Qed.
 
 End Combined.
 
+Inductive aval : aexp -> Prop :=
+  av_num : forall n, aval (ANum n).
+
+Reserved Notation " t '/' st '==>a' t' " (at level 40, st at level 39).
+
+Inductive astep : state -> aexp -> aexp -> Prop :=
+  | AS_Id : forall st i,
+      AId i / st ==>a ANum (st i)
+  | AS_Plus : forall st n1 n2,
+      APlus (ANum n1) (ANum n2) / st ==>a ANum (n1 + n2)
+  | AS_Plus1 : forall st a1 a1' a2,
+      a1 / st ==>a a1' ->
+      (APlus a1 a2) / st ==>a (APlus a1' a2)
+  | AS_Plus2 : forall st v1 a2 a2',
+      aval v1 ->
+      a2 / st ==>a a2' ->
+      (APlus v1 a2) / st ==>a (APlus v1 a2')
+  | AS_Minus : forall st n1 n2,
+      (AMinus (ANum n1) (ANum n2)) / st ==>a (ANum (minus n1 n2))
+  | AS_Minus1 : forall st a1 a1' a2,
+      a1 / st ==>a a1' ->
+      (AMinus a1 a2) / st ==>a (AMinus a1' a2)
+  | AS_Minus2 : forall st v1 a2 a2',
+      aval v1 ->
+      a2 / st ==>a a2' ->
+      (AMinus v1 a2) / st ==>a (AMinus v1 a2')
+  | AS_Mult : forall st n1 n2,
+      (AMult (ANum n1) (ANum n2)) / st ==>a (ANum (mult n1 n2))
+  | AS_Mult1 : forall st a1 a1' a2,
+      a1 / st ==>a a1' ->
+      (AMult (a1) (a2)) / st ==>a (AMult (a1') (a2))
+  | AS_Mult2 : forall st v1 a2 a2',
+      aval v1 ->
+      a2 / st ==>a a2' ->
+      (AMult v1 a2) / st ==>a (AMult v1 a2')
+
+    where " t '/' st '==>a' t' " := (astep st t t').
+
+  Reserved Notation " t '/' st '==>b' t' " (at level 40, st at level 39).
+
+  Inductive bstep : state -> bexp -> bexp -> Prop :=
+  | BS_Eq : forall st n1 n2,
+      (BEq (ANum n1) (ANum n2)) / st ==>b
+      (if (beq_nat n1 n2) then BTrue else BFalse)
+  | BS_Eq1 : forall st a1 a1' a2,
+      a1 / st ==>a a1' ->
+      (BEq a1 a2) / st ==>b (BEq a1' a2)
+  | BS_Eq2 : forall st v1 a2 a2',
+      aval v1 ->
+      a2 / st ==>a a2' ->
+      (BEq v1 a2) / st ==>b (BEq v1 a2')
+  | BS_LtEq : forall st (n1 n2 : nat),
+      (BLe (ANum n1) (ANum n2)) / st ==>b
+               (if (ble_nat n1 n2) then BTrue else BFalse)
+  | BS_LtEq1 : forall st a1 a1' a2,
+      a1 / st ==>a a1' ->
+      (BLe a1 a2) / st ==>b (BLe a1' a2)
+  | BS_LtEq2 : forall st v1 a2 a2',
+      aval v1 ->
+      a2 / st ==>a a2' ->
+      (BLe v1 a2) / st ==>b (BLe v1 (a2'))
+  | BS_NotTrue : forall st,
+      (BNot BTrue) / st ==>b BFalse
+  | BS_NotFalse : forall st,
+      (BNot BFalse) / st ==>b BTrue
+  | BS_NotStep : forall st b1 b1',
+      b1 / st ==>b b1' ->
+      (BNot b1) / st ==>b (BNot b1')
+  | BS_AndTrueTrue : forall st,
+      (BAnd BTrue BTrue) / st ==>b BTrue
+  | BS_AndTrueFalse : forall st,
+      (BAnd BTrue BFalse) / st ==>b BFalse
+  | BS_AndFalse : forall st b2,
+      (BAnd BFalse b2) / st ==>b BFalse
+  | BS_AndTrueStep : forall st b2 b2',
+      b2 / st ==>b b2' ->
+      (BAnd BTrue b2) / st ==>b (BAnd BTrue b2')
+  | BS_AndStep : forall st b1 b1' b2,
+      b1 / st ==>b b1' ->
+      (BAnd b1 b2) / st ==>b (BAnd b1' b2)
+
+  where " t '/' st '==>b' t' " := (bstep st t t').
+
+Reserved Notation " t '/' st '==>' t' '/' st' "
+                  (at level 40, st at level 39, t' at level 39).
+
+Inductive cstep : (com * state) -> (com * state) -> Prop :=
+  | CS_AssStep : forall st i a a',
+      a / st ==>a a' ->
+      (i ::= a) / st ==> (i ::= a') / st
+  | CS_Ass : forall st i n,
+      (i ::= (ANum n)) / st ==> SKIP / (update st i n)
+  | CS_SeqStep : forall st c1 c1' st' c2,
+      c1 / st ==> c1' / st' ->
+      (c1 ;; c2) / st ==> (c1' ;; c2) / st'
+  | CS_SeqFinish : forall st c2,
+      (SKIP ;; c2) / st ==> c2 / st
+  | CS_IfTrue : forall st c1 c2,
+      IFB BTrue THEN c1 ELSE c2 FI / st ==> c1 / st
+  | CS_IfFalse : forall st c1 c2,
+      IFB BFalse THEN c1 ELSE c2 FI / st ==> c2 / st
+  | CS_IfStep : forall st b b' c1 c2,
+      b / st ==>b b' ->
+          IFB b THEN c1 ELSE c2 FI / st 
+      ==> (IFB b' THEN c1 ELSE c2 FI) / st
+  | CS_While : forall st b c1,
+          (WHILE b DO c1 END) / st
+      ==> (IFB b THEN (c1;; (WHILE b DO c1 END)) ELSE SKIP FI) / st
+
+  where " t '/' st '==>' t' '/' st' " := (cstep (t,st) (t',st')).
+
+Module CImp.
+
+Inductive com : Type :=
+  | CSkip : com
+  | CAss : id -> aexp -> com
+  | CSeq : com -> com -> com
+  | CIf : bexp -> com -> com -> com
+  | CWhile : bexp -> com -> com
+  | CPar : com -> com -> com.
+
+Notation "'SKIP'" :=
+  CSkip.
+Notation "x '::=' a" :=
+  (CAss x a) (at level 60).
+Notation "c1 ;; c2" :=
+  (CSeq c1 c2) (at level 80, right associativity).
+Notation "'WHILE' b 'DO' c 'END'" :=
+  (CWhile b c) (at level 80, right associativity).
+Notation "'IFB' b 'THEN' c1 'ELSE' c2 'FI'" :=
+  (CIf b c1 c2) (at level 80, right associativity).
+Notation "'PAR' c1 'WITH' c2 'END'" :=
+  (CPar c1 c2) (at level 80, right associativity).
+
+Inductive cstep : (com * state)  -> (com * state) -> Prop :=
+    (* Old part *)
+  | CS_AssStep : forall st i a a',
+      a / st ==>a a' ->
+      (i ::= a) / st ==> (i ::= a') / st
+  | CS_Ass : forall st i n,
+      (i ::= (ANum n)) / st ==> SKIP / (update st i n)
+  | CS_SeqStep : forall st c1 c1' st' c2,
+      c1 / st ==> c1' / st' ->
+      (c1 ;; c2) / st ==> (c1' ;; c2) / st'
+  | CS_SeqFinish : forall st c2,
+      (SKIP ;; c2) / st ==> c2 / st
+  | CS_IfTrue : forall st c1 c2,
+      (IFB BTrue THEN c1 ELSE c2 FI) / st ==> c1 / st
+  | CS_IfFalse : forall st c1 c2,
+      (IFB BFalse THEN c1 ELSE c2 FI) / st ==> c2 / st
+  | CS_IfStep : forall st b b' c1 c2,
+      b /st ==>b b' ->
+          (IFB b THEN c1 ELSE c2 FI) / st 
+      ==> (IFB b' THEN c1 ELSE c2 FI) / st
+  | CS_While : forall st b c1,
+          (WHILE b DO c1 END) / st 
+      ==> (IFB b THEN (c1;; (WHILE b DO c1 END)) ELSE SKIP FI) / st
+  | CS_Par1 : forall st c1 c1' c2 st',
+      c1 / st ==> c1' / st' ->
+      (PAR c1 WITH c2 END) / st ==> (PAR c1' WITH c2 END) / st'
+  | CS_Par2 : forall st c1 c2 c2' st',
+      c2 / st ==> c2' / st' ->
+      (PAR c1 WITH c2 END) / st ==> (PAR c1 WITH c2' END) / st'
+  | CS_ParDone : forall st,
+      (PAR SKIP WITH SKIP END) / st ==> SKIP / st
+  where " t '/' st '==>' t' '/' st' " := (cstep (t,st) (t',st')).
+
+Definition cmultistep := multi cstep.
+
+Notation " t '/' st '==>*' t' '/' st' " :=
+   (multi cstep  (t,st) (t',st'))
+   (at level 40, st at level 39, t' at level 39).
+
+Definition par_loop : com :=
+  PAR
+    Y ::= ANum 1
+  WITH
+    WHILE BEq (AId Y) (ANum 0) DO
+      X ::= APlus (AId X) (ANum 1)
+    END
+  END.
+
+(* Exercise: 3 stars, optional (par_body_n__Sn) *)
+Lemma par_body_n__Sn : forall n st,
+  st X = n /\ st Y = 0 ->
+  par_loop / st ==>* par_loop / (update st X (S n)).
+Proof.
+  intros n st [stXn stY0].
+    eapply multi_step. apply CS_Par2. apply CS_While.
+    eapply multi_step. apply CS_Par2. apply CS_IfStep.
+      apply BS_Eq1. apply AS_Id.
+    eapply multi_step. apply CS_Par2. apply CS_IfStep.
+      apply BS_Eq.
+    eapply multi_step. rewrite stY0. simpl. apply CS_Par2.
+      apply CS_IfTrue.
+    eapply multi_step. apply CS_Par2. apply CS_SeqStep.
+      apply CS_AssStep. apply AS_Plus1. apply AS_Id.
+    eapply multi_step. apply CS_Par2. apply CS_SeqStep.
+      apply CS_AssStep. apply AS_Plus.
+    eapply multi_step. apply CS_Par2. apply CS_SeqStep. apply CS_Ass.
+    eapply multi_step. apply CS_Par2. apply CS_SeqFinish.
+    rewrite stXn. rewrite <- plus_n_Sm. rewrite <- plus_n_O. constructor.
+Qed.
+
+(* END par_body_n__Sn. *)
